generational/spec/GC.Gen.Cheney.fst
@@ -501,10 +501,14 @@ private let promote_object_preserves_objects_part1
     let dst_obj : obj_addr = alloc_res.obj_out in
     WriteBody.copy_fields_preserves_objects_aux minor alloc_res.heap_out obj dst_obj 0 wz;
     promote_object_success minor major obj fp wz;
+    AllocLemmas.alloc_spec_preserves_wfh_part1 major fp wz;
+    WriteBody.copy_fields_preserves_wfh_part1 minor alloc_res.heap_out obj dst_obj wz;
     let copied = WriteBody.copy_fields minor alloc_res.heap_out obj dst_obj 0 wz in
     let tag = minor_tag minor obj in
     minor_tag_bound minor obj;
-    set_promoted_tag_preserves_objects copied dst_obj tag
+    zero_promote_padding_preserves_objects copied dst_obj wz;
+    let padded = zero_promote_padding copied dst_obj wz in
+    set_promoted_tag_preserves_objects padded dst_obj tag
   end
 
 #pop-options
